\section{\texorpdfstring{Finding $w_1\otimes v_k$}{Finding w\_1 tensor v\_k}}\label{sec:w_1tensorv_k}
Using the bases $(s_k \mid 0\leq k\leq n+2)$ of \cref{eq:s_kbasisres}, $(t_k \mid 0\leq k\leq n)$ of \cref{eq:t_kbasisres}, and $(u_k \mid 0\leq k\leq n-2)$ of \cref{eq:u_kbasisres}, we see that
\begin{align*}
  &\dfrac{2(k+1)(n+1-k)}{(n+1)(n+2)}s_{k+1} - \dfrac{2(n-2k)}{n(n+2)}t_k - \dfrac{4}{n(n+1)}u_{k-1}\\
                                   &= \dfrac{2(k+1)(n+1-k)}{(n+1)(n+2)}\Bigl( w_0\otimes v_{k+1} + w_1\otimes v_{k} + w_2\otimes v_{k-1} \Bigr) \\*
                                   &\phantom{{}={}}{} - \dfrac{2(n-2k)}{n(n+2)}\Bigl( (k+1)w_0\otimes v_{k+1} - \dfrac{n-2k}{2}w_1\otimes v_k \\*
                                   &\phantom{{}={}-{}}{} + (k-1-n)w_2\otimes v_{k-1} \Bigr) \\*
                                   &\phantom{{}={}}{} - \dfrac{4}{n(n+1)}\Bigl( \dfrac{k(k+1)}{2}w_0\otimes v_{k+1} - \dfrac{k(n-k)}{2}w_1\otimes v_k \\*
                                   &\phantom{{}={}+{}}{}+ \dfrac{(n-k+1)(n-k)}{2}w_2\otimes v_{k-1} \Bigr) \\
  &= \dfrac{
    \biggl(\splitfrac{2(k+1)(n+1-k)n-2(n-2k)(k+1)(n+1)}{{}-2k(k+1)(n+2)}\biggr)
    }{n(n+1)(n+2)}w_0\otimes v_{k+1} \\*
  &\phantom{{}={}}{} + \dfrac{
    \biggl(\splitfrac{2(k+1)(n+1-k)n+(n-2k)(n-2k)(n+1)}{{}+2k(n-k)(n+2)}\biggr)
    }
    {n(n+1)(n+2)}w_1\otimes v_k \\*
  &\phantom{{}={}}{} + \dfrac{
    \biggl(\splitfrac{2(k+1)(n+1-k)n-2(n-2k)(k-1-n)(n+1)}{{}-2(n-k+1)(n-k)(n+2)}\biggr)
    }
    {n(n+1)(n+2)}w_2\otimes v_{k-1} \\
  &= 2(k+1)\dfrac{
    (n+1-k)n-(n-2k)(n+1)-k(n+2)
    }
    {n(n+1)(n+2)}w_0\otimes v_{k+1} \\*
  &\phantom{{}={}}{} + \dfrac{
    \biggl(\splitfrac{2(k+1)(n+1-k)n+(n-2k)(n-2k)(n+1)}{{}+2k(n-k)(n+2)}\biggr)
    }
    {n(n+1)(n+2)}w_1\otimes v_k \\*
  &\phantom{{}={}}{} + 2(n+1-k)\dfrac{
    (k+1)n + (n-2k)(n+1) - (n-k)(n+2)
    }
    {n(n+1)(n+2)}w_2\otimes v_{k-1}.
\end{align*}
Now we note that
\begin{align*}
  (n+1-k)n&-(n-2k)(n+1)-k(n+2) \\
          &= n\Bigl( (n+1-k)-(n-2k)-k \Bigr)-(n-2k)-2k \\
          &= n-(n-2k)-2k = 0,
\end{align*}
and
\begin{align*}
  (k+1)n&+(n-2k)(n+1)-(n-k)(n+2) \\
        &= n\Bigl( (k+1)+(n-2k) - (n-k) \Bigr) + (n-2k) - 2(n-k)\\
  &= n + n-2k -2n+2k = 0,
\end{align*}
while
\begin{align*}
  &2(k+1)(n+1-k)n + (n-2k)(n-2k)(n+1)+2k(n-k)(n+2) \\
  &= n\Bigl( 2(k+1)(n+1-k) + (n-2k)(n+1) + 2k(n-k) \Bigr) \\*
  &\phantom{{}={}}{} - 2k(n-2k)(n+1) + 4k(n-k) \\
  &= n\Bigl( 2(k+1)(n+1-k) + (n-2k)(n+1) + 2k(n-k) \Bigr) \\*
  &\phantom{{}={}}{} - 2kn(n-2k) - 2k(n-2k) + 4k(n-k) \\
  &= n\Bigl( 2(k+1)(n+1-k) + (n-2k)(n+1) + 2k(n-k) \Bigr) \\*
  &\phantom{{}={}}{} - 2kn(n-2k) + 2kn \\
  &= n\Bigl( 2(k+1)(n+1-k) + (n-2k)(n+1) + 2k(n-k) - 2k(n-2k) \\*
  &\phantom{{}={}n\Bigl()}{} + 2k \Bigr),
\end{align*}
where
\begin{align*}
  &2(k+1)(n+1-k) + (n-2k)(n+1) + 2k(n-k) - 2k(n-2k) + 2k \\
  &= (n+1)\Bigl( 2(k+1) + (n-2k) \Bigr) - 2k(k+1) \\*
  &\phantom{{}={}}{} + 2k\Bigl( (n-k) - (n-2k) + 1\Bigr) \\
  &= (n+1)(n+2) - 2k(k+1) + 2k(k+1) \\
  &= (n+1)(n+2),
\end{align*}
so
\begin{align*}
  &2(k+1)(n+1-k)n + (n-2k)(n-2k)(n+1)+2k(n-k)(n+2) \\
  &= n(n+1)(n+2).
\end{align*}
Thus we see that
\begin{align*}
  &\dfrac{2(k+1)(n+1-k)}{(n+1)(n+2)}s_{k+1} - \dfrac{2(n-2k)}{n(n+2)}t_k - \dfrac{4}{n(n+1)}u_{k-1}\\
  &= 0 + \dfrac{n(n+1)(n+2)}{n(n+1)(n+2)}w_1\otimes v_k + 0 \\
  &= w_1\otimes v_k
\end{align*}
giving us \cref{eq:w_1tensorv_k}. 

Likewise for $n\geq 1$, we get that
\begin{align*}
  \dfrac{2}{n+2}(s_1-t_0) &= \dfrac{2}{n+2}\Bigl( w_0\otimes v_1 + w_1\otimes v_0 - w_0\otimes v_1 + \dfrac{n}{2}w_1\otimes v_0 \Bigr) \\
  &= \dfrac{2}{n+2}\dfrac{n+2}{2}w_1\otimes v_0 \\
  &= w_1\otimes v_0
\end{align*}
and
\begin{align*}
  \dfrac{2}{n+2}(s_{n+1}+t_n) &= \dfrac{2}{n+2}\Bigl( w_2\otimes v_{n+1} + w_1\otimes v_n + \dfrac{n}{2}w_1\otimes v_n - w_2\otimes v_{n-1} \Bigr)\\
                              &= \dfrac{2}{n+2}\dfrac{n+2}{2} w_1\otimes v_n \\
  &= w_1\otimes v_n
\end{align*}
giving us \cref{eq:special_cases_w_1tensorv_k}.
%%% Local Variables:
%%% mode: latex
%%% TeX-master: "../main"
%%% End:
