\section{\texorpdfstring{$F_3,F_+,F_-$ in terms of $E_+,E_-,D_0,D_+,D_-$}{F\_3,F\_+,F\_- in terms of E\_+,E\_-,D\_0,D\_+,D\_-}}\label{sec:Factions}

We have already seen that
\begin{align*}
  F_3 \xi = \sqrt{\ell^2-m^2} D_- \xi - m D_0 \xi - \sqrt{(\ell+1)^2-m^2} D_+ \xi
\end{align*}
for $\xi\in R_{\ell,m}$ by using \cref{eq:F_3action} and the definition of how we expanded $D_0$, $D_+$, and $D_-$ to maps on all of $M$. Now we get by \cref{eq:lierels,eq:E+andE-} that
\begin{align*}
  F_+ \xi &= [F_3,H_+] \xi = F_3H_+ \xi - H_+F_3 \xi \\
          &= \sqrt{(\ell+m+1)(\ell-m)}F_3E_+ \xi - \sqrt{\ell^2-m^2} H_+D_- \xi + m H_+D_0 \xi \\*
          &\phantom{{}={}}{} + \sqrt{(\ell+1)^2-m^2} H_+D_+ \xi \\
          &= \sqrt{(\ell+m+1)(\ell-m)}\Bigl( \sqrt{\ell^2-(m+1)^2} D_-E_+ \xi - (m+1) D_0E_+ \xi \\*
          &\phantom{{}={}\sqrt{(\ell+m+1)(\ell-m)}()}{} - \sqrt{(\ell+1)^2-(m+1)^2} D_+E_+ \xi \Bigr) \\*
          &\phantom{{}={}}{} - \sqrt{\ell^2-m^2} \sqrt{((\ell-1)+m+1)((\ell-1)-m)} E_+D_- \xi \\*
          &\phantom{{}={}}{} + m \sqrt{(\ell+m+1)(\ell-m)}E_+D_0 \xi \\*
          &\phantom{{}={}}{} + \sqrt{(\ell+1)^2-m^2}\sqrt{((\ell+1)+m+1)((\ell+1)-m)} E_+D_+ \xi \\
          &= \sqrt{(\ell+m+1)(\ell-m)}\Bigl( \sqrt{\ell^2-(m+1)^2} D_-E_+ \xi - (m+1) D_0E_+ \xi \\*
          &\phantom{{}={}\sqrt{(\ell+m+1)(\ell-m)}()}{} - \sqrt{(\ell+1)^2-(m+1)^2} D_+E_+ \xi \Bigr) \\*
          &\phantom{{}={}}{} - \sqrt{\ell^2-m^2} \sqrt{(\ell+ml)(\ell-m-1)} D_-E_+ \xi \\*
          &\phantom{{}={}}{} + m \sqrt{(\ell+m+1)(\ell-m)}D_0E_+ \xi \\*
          &\phantom{{}={}}{} + \sqrt{(\ell+1)^2-m^2}\sqrt{(\ell+m+2)(\ell-m+1)} D_+E_+ \xi \\
          &= \Bigl( \sqrt{(\ell+m+1)(\ell-m)(\ell^2-(m+1)^2)} \\*
          &\phantom{{}={}()}{} - \sqrt{(l^2-m^2)(l+m)(l-m-1)} \Bigr)D_-E_+ \xi \\*
          &\phantom{{}={}}{} - \sqrt{(\ell+m+1)(\ell-m)}D_0E_+\xi \\*
          &\phantom{{}={}}{} + \Bigl( \sqrt{((\ell+1)^2-m^2)(\ell+m+2)(\ell-m+1)} \\*
          &\phantom{{}={}()}{} - \sqrt{(\ell+m+1)(\ell-m)((\ell+1)^2-(m+1)^2)}\Bigr)D_+E_+\xi.
\end{align*}
By pure algebraic manipulation note that \todo{I have checked this in Mathematica, but I would prefer not to write this out, although I can do it later if necessary}
\begin{align*}
  &\sqrt{(\ell+m+1)(\ell-m)(\ell^2-(m+1)^2)} - \sqrt{(l^2-m^2)(l+m)(l-m-1)} \\
  &= \sqrt{(\ell-m)(\ell-m-1)}
\end{align*}
and
\begin{align*}
  &\sqrt{((\ell+1)^2-m^2)(\ell+m+2)(\ell-m+1)} \\*
  &\phantom{{}={}}{} - \sqrt{(\ell+m+1)(\ell-m)((\ell+1)^2-(m+1)^2)} \\
  &= \sqrt{(\ell+m+1)((\ell+m+2))},
\end{align*}
so we get that
\begin{align*}
  F_+ \xi &= \sqrt{(\ell-m)(\ell-m-1)} D_-E_+ \xi - \sqrt{(\ell+m+1)(\ell-m)} D_0E_+\xi \\*
  &\phantom{{}={}}{} - \sqrt{(\ell+m+1)(\ell+m+2)} D_+E_+\xi.
\end{align*}


%%% Local Variables:
%%% mode: latex
%%% TeX-master: "../main"
%%% End:
